

# Darboux's formula

Emil Kerimov

## 1 Darboux's formula

Let  $\phi(t)$  be a polynomial of degree  $n$  and  $f(x)$  is an analytic function then,

**Theorem 1.1.**

$$\sum_{m=0}^n (-1)^m (z-a)^m \left[ \phi^{(n-m)}(1) f^{(m)}(z) - \phi^{(n-m)}(0) f^{(m)}(a) \right] = (-1)^n (z-a)^{n+1} \int_0^1 \phi(t) f^{(n+1)}[a+t(z-a)] dt \quad (1)$$

*Proof*

For  $n = 0$  we have  $\phi(t) = c$  then

$$LHS_0 = c [f(z) - f(a)]$$
$$RHS_0 = (z-a) \int_0^1 c f^{(1)}[a+t(z-a)] dt$$

After a change of variables  $u = a + t(z-a)$ ,  $du = dt(z-a)$  we get

$$RHS_0 = c \int_a^z f^{(1)}(u) du = c [f(u)] \Big|_{u=a}^{u=z} = c [f(z) - f(a)] = LHS_0$$

For  $n > 0$

$$RHS_n = (-1)^n (z-a)^{n+1} \int_0^1 \phi(t) f^{(n+1)}[a+t(z-a)] dt$$

Using integration by parts  $\int_{t=0}^1 uv' = uv \Big|_{t=0}^1 - \int_{t=0}^1 u'v$ , with  $u = \phi(t)$ , and  $v' = f^{(n+1)}(a+t(z-a))$

$$RHS_n = (-1)^n (z-a)^{n+1} \left[ \phi(t) \frac{f^{(n)}[a+t(z-a)]}{(z-a)} \Big|_{t=0}^{t=1} - \int_0^1 \phi'(t) \frac{f^{(n)}[a+t(z-a)]}{(z-a)} dt \right]$$

Evaluating the first definite integral and multiplying by  $(z-a)$

$$RHS_n = (-1)^n (z-a)^n \left[ \phi(1) f^{(n)}(z) - \phi(0) f^{(n)}(a) - \int_0^1 \phi'(t) f^{(n)}[a+t(z-a)] dt \right]$$

Moving the second integral out to it's own term

$$RHS_n = (-1)^n (z-a)^n \left[ \phi(1)f^{(n)}(z) - \phi(0)f^{(n)}(a) \right] + (-1)^{n-1} (z-a)^n \int_0^1 \phi'(t)f^{(n)}[a+t(z-a)] dt$$

Repeating the integration by parts process we get

$$\begin{aligned} RHS_n &= (-1)^n (z-a)^n \left[ \phi(1)f^{(n)}(z) - \phi(0)f^{(n)}(a) \right] \\ &+ (-1)^{n-1} (z-a)^{n-1} \left[ \phi^{(1)}(1)f^{(n-1)}(z) - \phi^{(1)}(0)f^{(n-1)}(a) \right] \\ &+ (-1)^{n-2} (z-a)^{n-1} \int_0^1 \phi^{(2)}(t)f^{(n-1)}[a+t(z-a)] dt \end{aligned}$$

Repeating the integration by parts  $n$ -times until  $\phi^{(n+1)}(t) = 0$  we get

$$RHS_n = \sum_{k=0}^n (-1)^{n-k} (z-a)^{n-k} \left[ \phi^{(k)}(1)f^{(n-k)}(z) - \phi^{(k)}(0)f^{(n-k)}(a) \right] + 0$$

Changing the index of summation  $m = n - k$

$$RHS_n = \sum_{m=0}^n (-1)^m (z-a)^m \left[ \phi^{(n-m)}(1)f^{(m)}(z) - \phi^{(n-m)}(0)f^{(m)}(a) \right]$$

Therefore we get

$$\begin{aligned} \sum_{m=0}^n (-1)^m (z-a)^m \left[ \phi^{(n-m)}(1)f^{(m)}(z) - \phi^{(n-m)}(0)f^{(m)}(a) \right] = \\ (-1)^n (z-a)^{n+1} \int_0^1 \phi(t)f^{(n+1)}[a+t(z-a)] dt \end{aligned}$$

## 2 Taylor's formula

Set  $\phi(t) = (t-1)^n$  into Darnoux's formula to obtain Taylor's formula.

**Theorem 2.1.**

$$f(z) = \sum_{m=0}^n \frac{(z-a)^m f^{(m)}(a)}{m!} + (-1)^n \frac{(z-a)^{n+1}}{n!} \int_0^1 (t-1)^n f^{(n+1)}[a+t(z-a)] dt \quad (2)$$

*Proof*

*Starting from Darboux's formula ??*

$$\begin{aligned} \sum_{m=0}^n (-1)^m (z-a)^m \left[ \phi^{(n-m)}(1) f^{(m)}(z) - \phi^{(n-m)}(0) f^{(m)}(a) \right] = \\ (-1)^n (z-a)^{n+1} \int_0^1 \phi(t) f^{(n+1)}[a+t(z-a)] dt \end{aligned}$$

*Setting  $\phi(t) = (t-1)^n$ , which is an  $n$ -degree polynomial*

*Note that  $\phi^{(k)}(t) = \frac{n!}{(n-k)!} (t-1)^{n-k}$  for  $k \leq n$ , therefore*

$$\begin{aligned} \phi^{(k)}(0) &= \frac{n!}{(n-k)!} (-1)^{n-k} \quad \text{for } k \leq n \\ \phi^{(k)}(1) &= 0 \quad \text{for } k < n \\ \phi^{(n)}(1) &= n! \end{aligned}$$

$$\begin{aligned} \sum_{m=1}^n (-1)^m (z-a)^m \left[ 0 - \frac{n!(-1)^m}{(m)!} f^{(m)}(a) \right] + (-1)^0 (z-a)^0 \left[ n! f^{(0)}(z) - n! f^{(0)}(a) \right] \\ = (-1)^n (z-a)^{n+1} \int_0^1 (t-1)^n f^{(n+1)}[a+t(z-a)] dt \end{aligned}$$

*Simplifying and dividing by  $n!$*

$$\begin{aligned} - \sum_{m=1}^n \frac{(z-a)^m}{m!} f^{(m)}(a) + [f(z) - f(a)] \\ = (-1)^n \frac{(z-a)^{n+1}}{n!} \int_0^1 (t-1)^n f^{(n+1)}[a+t(z-a)] dt \end{aligned}$$

*Rearranging*

$$f(z) = f(a) + \sum_{m=1}^n \frac{(z-a)^m}{m!} f^{(m)}(a) + (-1)^n \frac{(z-a)^{n+1}}{n!} \int_0^1 (t-1)^n f^{(n+1)}[a+t(z-a)] dt$$

*Adding the extra term into the summation to finish the proof*

$$f(z) = \sum_{m=0}^n \frac{(z-a)^m}{m!} f^{(m)}(a) + (-1)^n \frac{(z-a)^{n+1}}{n!} \int_0^1 (t-1)^n f^{(n+1)}[a+t(z-a)] dt$$

## 2.1 Infinite Series

**Theorem 2.2.** If  $|f^{(k)}(x)| \leq M$  and  $|z - a| \leq R \quad \forall x$  then

$$\boxed{f(z) = \sum_{m=0}^{\infty} \frac{(z-a)^m f^{(m)}(a)}{m!}} \quad (3)$$

*Proof*

Starting from Taylor's formula 2 and taking the limit as  $n$  approaches infinity

$$f(z) = \sum_{m=0}^{\infty} \frac{(z-a)^m f^{(m)}(a)}{m!} + \lim_{n \rightarrow \infty} (-1)^n \frac{(z-a)^{n+1}}{n!} \int_0^1 (t-1)^n f^{(n+1)}[a + t(z-a)] dt$$

Define the remainder term, and then we will show that it converges to 0

$$\begin{aligned} R_n &= (-1)^n \frac{(z-a)^{n+1}}{n!} \int_0^1 (t-1)^n f^{(n+1)}[a + t(z-a)] dt \\ |R_n| &= \left| (-1)^n \right| \cdot \left| \frac{(z-a)^{n+1}}{n!} \right| \cdot \left| \int_0^1 (t-1)^n f^{(n+1)}[a + t(z-a)] dt \right| \\ |R_n| &\leq \frac{|z-a|^{n+1}}{n!} \cdot \int_0^1 \left| (t-1)^n \right| \cdot \left| f^{(n+1)}[a + t(z-a)] \right| dt \end{aligned}$$

Using  $|f^{(k)}(x)| \leq M$

$$|R_n| \leq \frac{|z-a|^{n+1}}{n!} \cdot \int_0^1 |t-1|^n \cdot M dt$$

Using  $|z-a| \leq R$

$$|R_n| \leq \frac{R^{n+1}M}{n!} \cdot \int_0^1 |t-1|^n dt$$

Note that between  $0 \leq t \leq 1$ ,  $|t-1| \leq 1$ , therefore

$$|R_n| \leq \frac{R^{n+1}M}{n!}$$

Therefore since  $M$  and  $R$  are constant:

$$\lim_{n \rightarrow \infty} R_n \leq \lim_{n \rightarrow \infty} |R_n| \leq 0$$

Therefore

$$f(z) = \sum_{m=0}^{\infty} \frac{(z-a)^m f^{(m)}(a)}{m!}$$

### 3 Euler-Maclaurin formula

Set  $\phi(t) = B_n(x)$  into Darnoux's formula to obtain the Euler-Maclaurin formula, where  $B_n(x)$  is the Bernoulli polynomial<sup>1</sup>.

**Theorem 3.1.** *For any analytical  $g(x)$*

$$\boxed{\begin{aligned} w \sum_{j=0}^{r-1} g(a+jw) - \int_{x=a}^{a+rw} g(x)dx &= \frac{w}{2} (g(a) - g(a+rw)) + \\ &\sum_{k=1}^{\lfloor n/2 \rfloor} \frac{w^{2k} B_{2k}}{(2k)!} (g^{(2k-1)}(a+rw) - g^{(2k-1)}(a)) + R_{n,r} \\ R_{n,r} &= \frac{(-1)^{n+1} w^{n+1}}{n!} \int_0^r B_n(\{t\}) f^{(n+1)}(a+tw) dt \end{aligned}} \quad (4)$$

*Proof*

*Starting from Darboux's formula ??*

$$\begin{aligned} \sum_{m=0}^n (-1)^m (z-a)^m \left[ \phi^{(n-m)}(1) f^{(m)}(z) - \phi^{(n-m)}(0) f^{(m)}(a) \right] = \\ (-1)^n (z-a)^{n+1} \int_0^1 \phi(t) f^{(n+1)}[a+t(z-a)] dt \end{aligned}$$

*Setting  $\phi(t) = B_n(t)$ , which is an  $n$ -degree polynomial*

*Note that  $\phi^{(k)}(t) = \frac{n!}{(n-k)!} B_{n-k}(t)$  for  $k \leq n$ , therefore*

$$\begin{aligned} \phi^{(k)}(0) = \phi^{(k)}(1) &= \frac{n!}{(n-k)!} B_{n-k} \quad \text{for } k \leq n, k \neq 1 \\ \phi^{(1)}(0) = -\phi^{(1)}(1) &= B_1 \end{aligned}$$

*adjusting the indicies we get*

$$\begin{aligned} \phi^{(n-m)}(0) = \phi^{(n-m)}(1) &= \frac{n!}{m!} B_m \quad \text{for } n \geq m \geq 0, m \neq 1 \\ \phi^{(n-1)}(0) = B_1 &= -\phi^{(n-1)}(1) \end{aligned}$$

*Plugging these values into Darboux's formula, and removing the first two terms we get*

$$\begin{aligned} \sum_{m=2}^n (-1)^m (z-a)^m \left[ \frac{n!}{m!} B_m f^{(m)}(z) - \frac{n!}{m!} B_m f^{(m)}(a) \right] + n! B_0 (f(z) - f(a)) \\ + (-1)n! (z-a) \left( -B_1 f'(z) - B_1 f'(a) \right) = (-1)^n (z-a)^{n+1} \int_0^1 B_n(t) f^{(n+1)}[a+t(z-a)] dt \end{aligned}$$

---

<sup>1</sup> $B_n(x) = \sum_{k=0}^n \binom{n}{k} B_k x^{n-k}$ . See the Bernoulli number document for the full definition.

simplifying

$$\sum_{m=2}^n \frac{(-1)^m (z-a)^m B_m}{m!} (f^{(m)}(z) - f^{(m)}(a)) + B_0 (f(z) - f(a)) + (z-a) B_1 (f'(z) + f'(a)) = \frac{(-1)^n (z-a)^{n+1}}{n!} \int_0^1 B_n(t) f^{(n+1)}[a + t(z-a)] dt$$

To simplify notation let us define  $R_n^a$

$$R_n^a = \frac{(-1)^n (z-a)^{n+1}}{n!} \int_0^1 B_n(t) f^{(n+1)}[a + t(z-a)] dt$$

Therefore we get

$$\sum_{m=2}^n \frac{(-1)^m (z-a)^m B_m}{m!} (f^{(m)}(z) - f^{(m)}(a)) + B_0 (f(z) - f(a)) + (z-a) B_1 (f'(z) + f'(a)) = R_n^a$$

Plugging in  $B_0 = 1$  and  $B_1 = -\frac{1}{2}$

$$\sum_{m=2}^n \frac{(-1)^m (z-a)^m B_m}{m!} (f^{(m)}(z) - f^{(m)}(a)) + (f(z) - f(a)) - (z-a) \frac{1}{2} (f'(z) + f'(a)) = R_n^a$$

Adding  $(z-a)f'(a)$  to both sides and rearranging we get

$$(z-a)f'(a) = f(z) - f(a) - \frac{(z-a)}{2} (f'(z) - f'(a)) + \sum_{m=2}^n \frac{(-1)^m (z-a)^m B_m}{m!} (f^{(m)}(z) - f^{(m)}(a)) - R_n^a$$

Define  $w = z - a$  and  $g(x) = f'(x)$  therefore we get

$$wg(a) = \int_{x=a}^{a+w} g(x) dx - \frac{w}{2} (g(a+w) - g(a)) + \sum_{m=2}^n \frac{(-1)^m w^m B_m}{m!} (g^{(m-1)}(a+w) - g^{(m-1)}(a)) - R_n^a$$

Allowing  $a$  to be multiples of  $w$ ,  $a' = a + jw$  and summing over  $i$  we get

$$\begin{aligned} \sum_{j=0}^{r-1} wg(a+jw) &= \sum_{j=0}^{r-1} \int_{x=a+jw}^{a+(j+1)w} g(x) dx - \sum_{j=0}^{r-1} \frac{w}{2} (g(a+(j+1)w) - g(a+jw)) \\ &+ \sum_{j=0}^{r-1} \sum_{m=2}^n \frac{(-1)^m w^m B_m}{m!} (g^{(m-1)}(a+(j+1)w) - g^{(m-1)}(a+jw)) - \sum_{j=0}^{r-1} R_n^{a+jw} \end{aligned}$$

Simplify and evaluating the sums we get

$$\begin{aligned} w \sum_{j=0}^{r-1} g(a+jw) &= \int_{x=a}^{a+rw} g(x) dx - \frac{w}{2} (g(a+rw) - g(a)) \\ &+ \sum_{m=2}^n \frac{(-1)^m w^m B_m}{m!} (g^{(m-1)}(a+rw) - g^{(m-1)}(a)) - \sum_{j=0}^{r-1} R_n^{a+jw} \end{aligned}$$

*Rearranging*

$$w \sum_{j=0}^{r-1} g(a+jw) - \int_{x=a}^{a+rw} g(x)dx = \frac{w}{2} (g(a) - g(a+rw)) \\ + \sum_{m=2}^n \frac{(-1)^m w^m B_m}{m!} (g^{(m-1)}(a+rw) - g^{(m-1)}(a)) - \sum_{j=0}^{r-1} R_n^{a+jw}$$

Using the fact that  $B_{2n+1} = 0, n \geq 1$  we can simplify the sum using  $m = 2k$

$$w \sum_{j=0}^{r-1} g(a+jw) - \int_{x=a}^{a+rw} g(x)dx = \frac{w}{2} (g(a) - g(a+rw)) \\ + \sum_{k=1}^{\lfloor n/2 \rfloor} \frac{w^{2k} B_{2k}}{(2k)!} (g^{(2k-1)}(a+rw) - g^{(2k-1)}(a)) - \sum_{j=0}^{r-1} R_n^{a+jw}$$

*Recall the remainder term definition*

$$R_n^a = \frac{(-1)^n (z-a)^{n+1}}{n!} \int_0^1 B_n(t) f^{(n+1)}[a+t(z-a)] dt$$

*Plugging in the definition of  $w = (z-a)$  we get*

$$R_n^a = \frac{(-1)^n w^{n+1}}{n!} \int_0^1 B_n(t) f^{(n+1)}[a+tw] dt$$

*Define the new remainder term*

$$R_n = - \sum_{j=0}^{r-1} R_n^{a+jw}$$

*Plug in the definition of  $R_n^{a+jw}$  and simplify*

$$R_n = - \sum_{j=0}^{r-1} \frac{(-1)^n w^{n+1}}{n!} \int_0^1 B_n(t) f^{(n+1)}(a+jw+tw) dt$$

*Simplify the remainder term using the fractional operator  $\{x\}$*

$$R_{n,r} = \frac{(-1)^{n+1} w^{n+1}}{n!} \int_0^r B_n(\{t\}) f^{(n+1)}(a+tw) dt$$

### 3.1 Infinite Series

Note that as  $n$  approaches infinity, the remainder term goes to 0.

**Theorem 3.2.** *If  $|g^{(k)}(x)| \leq M \quad \forall x$  and  $a, w, M$  finite then*

$$\boxed{\lim_{n \rightarrow \infty} R_{n,r} = \lim_{n \rightarrow \infty} \frac{(-1)^{n+1} w^{n+1}}{n!} \int_0^r B_n(\{t\}) f^{(n+1)}(a+tw) dt = 0} \quad (5)$$

*Proof*

Starting from the definition of  $R_{n,r}$

$$\begin{aligned}\lim_{n \rightarrow \infty} R_n &= \lim_{n \rightarrow \infty} \frac{(-1)^{n+1} w^{n+1}}{n!} \int_0^r B_n(\{t\}) f^{(n+1)}(a + tw) dt = 0 \\ \lim_{n \rightarrow \infty} R_n &\leq \lim_{n \rightarrow \infty} |R_n| \\ |R_n| &\leq \frac{|w|^{n+1}}{n!} \int_0^r |B_n(\{t\})| M dt \leq \frac{|w|^{n+1} |B_n(t)| r M}{n!}\end{aligned}$$

Using  $\lim_{n \rightarrow \infty} \frac{B_n(x)}{n!} = 0$  from *BERNOULLI DOCUMENT TODO*

$$\lim_{n \rightarrow \infty} R_n \leq \lim_{n \rightarrow \infty} |R_n| = 0$$

### 3.2 Simple version

By specifying  $a = 0$  and  $w = 1$  we obtain an exact difference between the summation and the integral of any analytic function  $g(x)$ .

**Theorem 3.3.** *For any analytical  $g(x)$*

$$\begin{aligned}\sum_{j=0}^r g(j) - \int_{x=0}^r g(x) dx &= \frac{g(0) + g(r)}{2} + \sum_{k=1}^{\lfloor n/2 \rfloor} \frac{B_{2k}}{(2k)!} \left( g^{(2k-1)}(r) - g^{(2k-1)}(0) \right) + R_{n,r} \\ R_{n,r} &= \frac{(-1)^{n+1}}{n!} \int_0^r B_n(\{t\}) g^{(n)}(t) dt\end{aligned}$$

(6)

*Proof*

Starting from the Euler-Maclaurin formula

$$\begin{aligned}w \sum_{j=0}^{r-1} g(a + jw) - \int_{x=a}^{a+rw} g(x) dx &= \frac{w}{2} (g(a) - g(a + rw)) + \\ &\sum_{k=1}^{\lfloor n/2 \rfloor} \frac{w^{2k} B_{2k}}{(2k)!} \left( g^{(2k-1)}(a + rw) - g^{(2k-1)}(a) \right) + R_{n,r} \\ R_{n,r} &= \frac{(-1)^{n+1} w^{n+1}}{n!} \int_0^r B_n(\{t\}) g^{(n)}(a + tw) dt\end{aligned}$$

Plugging in  $a = 0$  and  $w = 1$  we get

$$\begin{aligned}\sum_{j=0}^{r-1} g(j) - \int_{x=0}^r g(x) dx &= \frac{1}{2} (g(0) - g(r)) + \sum_{k=1}^{\lfloor n/2 \rfloor} \frac{B_{2k}}{(2k)!} \left( g^{(2k-1)}(r) - g^{(2k-1)}(0) \right) + R_{n,r} \\ R_{n,r} &= \frac{(-1)^{n+1}}{n!} \int_0^r B_n(\{t\}) g^{(n)}(t) dt\end{aligned}$$

Adding  $g(r)$  to both sides

$$\sum_{j=0}^r g(j) - \int_{x=0}^r g(x) dx = \frac{g(0) + g(r)}{2} + \sum_{k=1}^{\lfloor n/2 \rfloor} \frac{B_{2k}}{(2k)!} \left( g^{(2k-1)}(r) - g^{(2k-1)}(0) \right) + R_{n,r}$$